Fix compilerProof by assuming input is not an sexp
A more sophisticated theorem might handle the sexp case, probably by
treating the sexp parser as an executable spec.

compiler/proofs/compilerProofScript.sml
@@ -12,6 +12,7 @@ val config_ok_def = Define`
   config_ok (cc:α compiler$config) mc ⇔
     env_rel prim_tenv cc.inferencer_config.inf_env ∧
     prim_tdecs = convert_decls cc.inferencer_config.inf_decls ∧
+    ¬cc.input_is_sexp ∧
     backend_config_ok cc.backend_config ∧ mc_conf_ok mc ∧ mc_init_ok cc.backend_config mc`;
 
 val initial_condition_def = Define`
@@ -20,6 +21,7 @@ val initial_condition_def = Define`
     (?ctMap. type_sound_invariant st.sem_st st.sem_env st.tdecs ctMap FEMPTY st.tenv) ∧
     env_rel st.tenv cc.inferencer_config.inf_env ∧
     st.tdecs = convert_decls cc.inferencer_config.inf_decls ∧
+    ¬cc.input_is_sexp ∧
     backend_config_ok cc.backend_config ∧ mc_conf_ok mc ∧ mc_init_ok cc.backend_config mc`;
 
 val parse_prog_correct = Q.store_thm("parse_prog_correct",
@@ -121,6 +123,8 @@ val compile_correct_gen = Q.store_thm("compile_correct_gen",
   rpt strip_tac
   \\ simp[compilerTheory.compile_def]
   \\ simp[parse_prog_correct]
+  \\ BasicProvers.CASE_TAC
+  >- fs[initial_condition_def]
   \\ BasicProvers.CASE_TAC
   \\ simp[semantics_def]
   \\ fs[initial_condition_def]
